RocqOfRust/examples/default/examples/custom/links/loops_free.v
@@ -22,25 +22,37 @@ Proof.
   run_symbolic.
 Defined.
 
-Instance run_get_or_zero (xs : array.t U32.t {| Integer.value := 4 |}) (i : Usize.t) :
+(* pub fn get_or_zero(xs: &[u32; 4], i: usize) -> u32 *)
+Instance run_get_or_zero
+    (xs : Ref.t Pointer.Kind.Ref (array.t U32.t {| Integer.value := 4 |}))
+    (i : Usize.t) :
   Run.Trait get_or_zero [] [] [φ xs; φ i] U32.t.
 Proof.
   constructor.
   run_symbolic.
 Defined.
 
-Instance run_eq2 (a b : array.t U32.t {| Integer.value := 2 |}) : Run.Trait eq2 [] [] [φ a; φ b] bool.
+(* pub fn eq2(a: &[u32; 2], b: &[u32; 2]) -> bool *)
+Instance run_eq2
+    (a : Ref.t Pointer.Kind.Ref (array.t U32.t {| Integer.value := 2 |}))
+    (b : Ref.t Pointer.Kind.Ref (array.t U32.t {| Integer.value := 2 |})) :
+  Run.Trait eq2 [] [] [φ a; φ b] bool.
 Proof.
   constructor.
   run_symbolic.
 Defined.
 
-Instance run_eq_pair (x y : Prod.t U32.t U32.t) : Run.Trait eq_pair [] [] [φ x; φ y] bool.
+(* pub fn eq_pair(x: (u32, u32), y: (u32, u32)) -> bool *)
+Instance run_eq_pair
+    (x : U32.t * U32.t)
+    (y : U32.t * U32.t) :
+  Run.Trait eq_pair [] [] [φ x; φ y] bool.
 Proof.
   constructor.
   run_symbolic.
 Defined.
 
+(* pub fn min3(a: u32, b: u32, c: u32) -> u32 *)
 Instance run_min3 (a b c : U32.t) : Run.Trait min3 [] [] [φ a; φ b; φ c] U32.t.
 Proof.
   constructor.
